grind: parameterising by primop table

src/Pipit.Context.Properties.fst
@@ -3,33 +3,34 @@
    them. *)
 module Pipit.Context.Properties
 
-open Pipit.Context.Base
-open Pipit.Context.Row
+module List = FStar.List.Tot
+module C = Pipit.Context.Base
+module R = Pipit.Context.Row
 
 (* Properties should only require one implicit unrolling of recursive definitions, and one implicit inversion *)
 #push-options "--fuel 1 --ifuel 1"
 
-let lemma_drop0 (c: context { List.length c > 0 }):
-  Lemma (ensures (drop1 c 0 == List.tl c)) = ()
+let lemma_drop0 (c: C.context 'a { List.length c > 0 }):
+  Lemma (ensures (C.drop1 c 0 == List.tl c)) = ()
 
-let lemma_lift0 (c: context) (t: Type):
-  Lemma (ensures (lift1 c 0 t == t :: c)) = ()
+let lemma_lift0 (c: C.context 'a) (t: 'a):
+  Lemma (ensures (C.lift1 c 0 t == t :: c)) = ()
 
 // XXX: these look like good candidates for SMT patterns but seem to cause flakiness
-let lemma_dropCons (c0: Type) (c': context) (i: index { 0 < i /\ i <= List.length c' }):
-  Lemma (ensures (drop1 (c0 :: c') i == c0 :: drop1 c' (i - 1)))
+let lemma_dropCons (c0: 'a) (c': C.context 'a) (i: C.index { 0 < i /\ i <= List.length c' }):
+  Lemma (ensures (C.drop1 (c0 :: c') i == c0 :: C.drop1 c' (i - 1)))
         = // [SMTPat (drop1 (c0 :: c') i)] =
   ()
 
-let lemma_liftCons (c0: Type) (c': context) (i: index { 0 < i /\ i <= List.length c' + 1}) (t: Type):
-  Lemma (ensures (lift1 (c0 :: c') i t == c0 :: lift1 c' (i - 1) t))
+let lemma_liftCons (c0: 'a) (c': C.context 'a) (i: C.index { 0 < i /\ i <= List.length c' + 1}) (t: 'a):
+  Lemma (ensures (C.lift1 (c0 :: c') i t == c0 :: C.lift1 c' (i - 1) t))
         = // [SMTPat (lift1 (c0 :: c') i t)] =
   ()
 
-let lemma_get_index_Cons (c0: Type) (c': context) (i1: index { has_index c' i1 }):
-  Lemma (ensures (get_index (c0 :: c') (i1 + 1) == get_index c' i1)) = ()
+let lemma_get_index_Cons (c0: 'a) (c': C.context 'a) (i1: C.index_lookup c'):
+  Lemma (ensures (C.get_index (c0 :: c') (i1 + 1) == C.get_index c' i1)) = ()
 
-let rec lemma_open_preserves_opt_index (c: context) (n: index { has_index c n }) (i: index { i <> n }): Lemma (opt_index c i == opt_index (open1' c n) (index_drop i n)) =
+let rec lemma_open_preserves_opt_index (c: C.context 'a) (n: C.index_lookup c) (i: C.index { i <> n }): Lemma (C.opt_index c i == C.opt_index (C.open1' c n) (C.index_drop i n)) =
   match c with
   | [] -> ()
   | _ :: c' ->
@@ -37,7 +38,7 @@ let rec lemma_open_preserves_opt_index (c: context) (n: index { has_index c n })
     then lemma_open_preserves_opt_index c' (n - 1) (i - 1)
     else ()
 
-let rec lemma_close_preserves_opt_index (c: context) (t: Type) (n: index { n <= List.length c }) (i: index): Lemma (opt_index c i == opt_index (close1' c t n) (index_lift i n)) =
+let rec lemma_close_preserves_opt_index (c: C.context 'a) (t: 'a) (n: C.index_insert c) (i: C.index): Lemma (C.opt_index c i == C.opt_index (C.close1' c t n) (C.index_lift i n)) =
   match c with
   | [] -> ()
   | _ :: c' ->
@@ -45,8 +46,8 @@ let rec lemma_close_preserves_opt_index (c: context) (t: Type) (n: index { n <= 
     then lemma_close_preserves_opt_index c' t (n - 1) (i - 1)
     else ()
 
-let rec lemma_close_contains (c: context) (t: Type) (n: index { n <= List.length c }): Lemma (opt_index (close1' c t n) n == Some t)
-  [SMTPat (opt_index (close1' c t n) n)] =
+let rec lemma_close_contains (c: C.context 'a) (t: 'a) (n: C.index_insert c): Lemma (C.opt_index (C.close1' c t n) n == Some t)
+  [SMTPat (C.opt_index (C.close1' c t n) n)] =
   match c with
   | [] -> ()
   | _ :: c' ->
@@ -54,7 +55,7 @@ let rec lemma_close_contains (c: context) (t: Type) (n: index { n <= List.length
     then lemma_close_contains c' t (n - 1)
     else ()
 
-let rec lemma_append_preserves_opt_index (c c': context) (n: index { has_index c n }): Lemma (opt_index c n == opt_index (append c c') n) =
+let rec lemma_append_preserves_opt_index (c c': C.context 'a) (n: C.index_lookup c): Lemma (C.opt_index c n == C.opt_index (C.append c c') n) =
   match c with
   | [] -> ()
   | _ :: c1' ->
@@ -62,8 +63,18 @@ let rec lemma_append_preserves_opt_index (c c': context) (n: index { has_index c
     then lemma_append_preserves_opt_index c1' c' (n - 1)
     else ()
 
-let rec lemma_lift_lift_commute (c: context) (i1: index { i1 <= List.length c }) (i2: index { i2 <= i1 }) (t1 t2: Type):
-  Lemma (ensures lift1 (lift1 c i1 t1) i2 t2 == lift1 (lift1 c i2 t2) (i1 + 1) t1) =
+
+let rec lemma_append_preserves_get_index (c c': C.context 'a) (n: C.index_lookup c): Lemma (n < List.length (C.append c c') /\ C.get_index c n == C.get_index (C.append c c') n) =
+  match c with
+  | [] -> ()
+  | _ :: c1' ->
+    List.append_length c c';
+    if n > 0
+    then (lemma_append_preserves_get_index c1' c' (n - 1))
+    else ()
+
+let rec lemma_lift_lift_commute (c: C.context 'a) (i1: C.index_insert c) (i2: C.index { i2 <= i1 }) (t1 t2: 'a):
+  Lemma (ensures C.lift1 (C.lift1 c i1 t1) i2 t2 == C.lift1 (C.lift1 c i2 t2) (i1 + 1) t1) =
   match c with
   | [] -> ()
   | c0 :: c' ->
@@ -73,8 +84,8 @@ let rec lemma_lift_lift_commute (c: context) (i1: index { i1 <= List.length c })
     else ()
 
 
-let rec lemma_drop_drop_commute (c: context) (i1: index { has_index c i1 }) (i2: index { i1 <= i2 /\ i2 < List.length c - 1 }):
-  Lemma (ensures drop1 (drop1 c i1) i2 == drop1 (drop1 c (i2 + 1)) i1) =
+let rec lemma_drop_drop_commute (c: C.context 'a) (i1: C.index_lookup c) (i2: C.index { i1 <= i2 /\ i2 < List.length c - 1 }):
+  Lemma (ensures C.drop1 (C.drop1 c i1) i2 == C.drop1 (C.drop1 c (i2 + 1)) i1) =
   match c with
   | [] -> ()
   | c0 :: c' ->
@@ -84,9 +95,9 @@ let rec lemma_drop_drop_commute (c: context) (i1: index { has_index c i1 }) (i2:
 
     else ()
 
-let rec lemma_drop_lift_eq (c: context) (i: index { i <= List.length c }) (t: Type):
-  Lemma (ensures drop1 (lift1 c i t) i == c)
-    [SMTPat (drop1 (lift1 c i t) i)] =
+let rec lemma_drop_lift_eq (c: C.context 'a) (i: C.index_insert c) (t: 'a):
+  Lemma (ensures C.drop1 (C.lift1 c i t) i == c)
+    [SMTPat (C.drop1 (C.lift1 c i t) i)] =
   match c with
   | [] -> ()
   | _ :: c' ->
@@ -94,9 +105,9 @@ let rec lemma_drop_lift_eq (c: context) (i: index { i <= List.length c }) (t: Ty
     then lemma_drop_lift_eq c' (i - 1) t
     else ()
 
-let rec lemma_lift_drop_eq (c: context) (i: index { i < List.length c }):
-  Lemma (ensures lift1 (drop1 c i) i (get_index c i) == c)
-    [SMTPat (lift1 (drop1 c i) i (get_index c i)) ]=
+let rec lemma_lift_drop_eq (c: C.context 'a) (i: C.index_lookup c):
+  Lemma (ensures C.lift1 (C.drop1 c i) i (C.get_index c i) == c)
+    [SMTPat (C.lift1 (C.drop1 c i) i (C.get_index c i)) ]=
   match c with
   | [] -> ()
   | _ :: c' ->
@@ -104,22 +115,22 @@ let rec lemma_lift_drop_eq (c: context) (i: index { i < List.length c }):
     then lemma_lift_drop_eq c' (i - 1)
     else ()
 
-let rec lemma_lift_drop_commute_le (c: context) (i1: index { has_index c i1 }) (i2: index { i2 <= i1 }) (t: Type):
-  Lemma (ensures (lift1 (drop1 c i1) i2 t == drop1 (lift1 c i2 t) (i1 + 1))) =
+let rec lemma_lift_drop_commute_le (c: C.context 'a) (i1: C.index_lookup c) (i2: C.index { i2 <= i1 }) (t: 'a):
+  Lemma (ensures (C.lift1 (C.drop1 c i1) i2 t == C.drop1 (C.lift1 c i2 t) (i1 + 1))) =
   match c with
   | [] -> ()
   | c0 :: c' ->
     if i1 > 0
-    then 
+    then
       if i2 > 0
       then
         lemma_lift_drop_commute_le c' (i1 - 1) (i2 - 1) t
       else ()
     else ()
 
-let rec lemma_lift_get_index (c: context) (i1: index { i1 <= List.length c }) (i2: index { i2 <= List.length c }) (t2: Type):
-  Lemma (ensures get_index (lift1 c i2 t2) i1 == (if i1 = i2 then t2 else get_index c (index_drop i1 i2)))
-        [SMTPat (get_index (lift1 c i2 t2) i1)] =
+let rec lemma_lift_get_index (c: C.context 'a) (i1: C.index_insert c) (i2: C.index_insert c) (t2: 'a):
+  Lemma (ensures C.get_index (C.lift1 c i2 t2) i1 == (if i1 = i2 then t2 else C.get_index c (C.index_drop i1 i2)))
+        [SMTPat (C.get_index (C.lift1 c i2 t2) i1)] =
   match c with
   | [] -> ()
   | _ :: c' ->
@@ -128,22 +139,22 @@ let rec lemma_lift_get_index (c: context) (i1: index { i1 <= List.length c }) (i
       lemma_lift_get_index c' (i1 - 1) (i2 - 1) t2
     else ()
 
-let lemma_lift_get_index_eq (c: context) (i: index { i <= List.length c }) (t: Type):
-  Lemma (ensures get_index (lift1 c i t) i == t)
-        [SMTPat (get_index (lift1 c i t) i)] =
+let lemma_lift_get_index_eq (c: C.context 'a) (i: C.index_insert c) (t: 'a):
+  Lemma (ensures C.get_index (C.lift1 c i t) i == t)
+        [SMTPat (C.get_index (C.lift1 c i t) i)] =
   lemma_lift_get_index c i i t
 
-let lemma_lift_get_index_gt (c: context) (i1: index { has_index c i1 }) (i2: index { i2 <= i1 }) (t2: Type):
-  Lemma (ensures get_index (lift1 c i2 t2) (i1 + 1) == get_index c i1) =
+let lemma_lift_get_index_gt (c: C.context 'a) (i1: C.index_lookup c) (i2: C.index { i2 <= i1 }) (t2: 'a):
+  Lemma (ensures C.get_index (C.lift1 c i2 t2) (i1 + 1) == C.get_index c i1) =
   lemma_lift_get_index c (i1 + 1) i2 t2
 
 // let lemma_lift_get_index_gt (c: context) (i1: index { i1 <= List.length c }) (i2: index { i2 <= i1 /\ i2 <= List.length c }) (t2: Type):
 //   Lemma (ensures get_index (lift1 c i2 t2) i1 == get_index c (i1 - 1)) =
 //   lemma_lift_get_index c i1 i2 t2
 
-let rec lemma_drop_get_index (c: context) (i1: index { has_index c i1 }) (i2: index { i2 < List.length c - 1 }):
-  Lemma (ensures get_index (drop1 c i1) i2 == get_index c (index_lift i2 i1))
-        [SMTPat (get_index (drop1 c i1) i2)] =
+let rec lemma_drop_get_index (c: C.context 'a) (i1: C.index_lookup c) (i2: C.index { i2 < List.length c - 1 }):
+  Lemma (ensures C.get_index (C.drop1 c i1) i2 == C.get_index c (C.index_lift i2 i1))
+        [SMTPat (C.get_index (C.drop1 c i1) i2)] =
   match c with
   | [] -> ()
   | _ :: c' ->
@@ -152,56 +163,59 @@ let rec lemma_drop_get_index (c: context) (i1: index { has_index c i1 }) (i2: in
       lemma_drop_get_index c' (i1 - 1) (i2 - 1)
     else ()
 
-let lemma_drop_get_index_gt (c: context) (i1: index { has_index c i1 }) (i2: index { i1 <= i2 /\ i2 < List.length c - 1 }):
-  Lemma (ensures get_index (drop1 c i1) i2 == get_index c (i2 + 1)) =
+let lemma_drop_get_index_gt (c: C.context 'a) (i1: C.index_lookup c) (i2: C.index { i1 <= i2 /\ i2 < List.length c - 1 }):
+  Lemma (ensures C.get_index (C.drop1 c i1) i2 == C.get_index c (i2 + 1)) =
   lemma_drop_get_index c i1 i2
 
-let lemma_drop_get_index_lt (c: context) (i1: index { has_index c i1 }) (i2: index { i2 < i1 /\ i2 < List.length c - 1 }):
-  Lemma (ensures get_index (drop1 c i1) i2 == get_index c i2) =
+let lemma_drop_get_index_lt (c: C.context 'a) (i1: C.index_lookup c) (i2: C.index { i2 < i1 /\ i2 < List.length c - 1 }):
+  Lemma (ensures C.get_index (C.drop1 c i1) i2 == C.get_index c i2) =
   lemma_drop_get_index c i1 i2
 
-let row_lift1_dropped (i: nat { i < List.length 'c }) (r: row (drop1 'c i)) (v: get_index 'c i): row 'c =
+let row_lift1_dropped (i: C.index_lookup 'c) (r: R.row (C.drop1 'c i)) (v: C.get_index 'c i): R.row 'c =
   lemma_lift_drop_eq 'c i;
-  row_lift1 r i v
+  R.lift1 r i v
 
-let row_zip2_lift1_dropped (i: nat { i < List.length 'c }) (rs: list (row (drop1 'c i))) (vs: list (get_index 'c i) { List.length rs == List.length vs }): (ret: list (row 'c) { List.length ret == List.length rs }) =
+let row_zip2_lift1_dropped (i: C.index_lookup 'c) (rs: list (R.row (C.drop1 'c i))) (vs: list (C.get_index 'c i) { List.length rs == List.length vs }): (ret: list (R.row 'c) { List.length ret == List.length rs }) =
   lemma_lift_drop_eq 'c i;
-  row_zip2_lift1 rs i vs
+  R.zip2_lift1 rs i vs
 
 let rec lemma_row_index_lift1_eq
-  (r: row 'c)
-  (i: index { i <= List.length 'c })
-  (v: 'a):
-  Lemma (ensures (row_index (lift1 'c i 'a) (row_lift1 r i v) i == v))
-        [SMTPat (row_index (lift1 'c i 'a) (row_lift1 r i v) i)] =
+  (#a: eqtype)
+  (r: R.row 'c)
+  (i: C.index_insert 'c)
+  (v: a):
+  Lemma (ensures (R.index (C.lift1 'c i a) (R.lift1 r i v) i == v))
+        [SMTPat (R.index (C.lift1 'c i a) (R.lift1 r i v) i)] =
   match 'c with
    | [] -> ()
    | c :: c' ->
-     let r': c & row c' = r in
+     let r': c & R.row c' = r in
      if i = 0
      then ()
      else lemma_row_index_lift1_eq (snd r') (i - 1) v
 
 let rec lemma_row_index_lift1
-  (r: row 'c)
-  (i: index { i <= List.length 'c })
-  (i': index { i' <= List.length 'c })
-  (v: 'a):
-  Lemma (ensures (row_index (lift1 'c i 'a) (row_lift1 r i v) i' == (if i = i' then v else (coerce_eq () (row_index 'c r (index_drop i' i))))))
-        [SMTPat (row_index (lift1 'c i 'a) (row_lift1 r i v) i')] =
+  (#a: eqtype)
+  (r: R.row 'c)
+  (i: C.index_insert 'c)
+  (i': C.index_insert 'c)
+  (v: a):
+  Lemma (ensures (R.index (C.lift1 'c i a) (R.lift1 r i v) i' == (if i = i' then v else (coerce_eq () (R.index 'c r (C.index_drop i' i))))))
+        [SMTPat (R.index (C.lift1 'c i a) (R.lift1 r i v) i')] =
   match 'c with
    | [] -> ()
    | c :: c' ->
-     let r': c & row c' = r in
+     let r': c & R.row c' = r in
      if i = 0 || i' = 0
      then ()
      else lemma_row_index_lift1 (snd r') (i - 1) (i' - 1) v
 
 let rec lemma_row_zip2_lift1_row_zip2_cons
-  (rows: list (row 'c))
-  (vs: list 'a { List.length rows == List.length vs }):
-  Lemma (ensures (row_zip2_lift1 rows 0 vs == row_zip2_cons vs rows))
-        [SMTPat (row_zip2_lift1 rows 0 vs)] =
+  (#a: eqtype)
+  (rows: list (R.row 'c))
+  (vs: list a { List.length rows == List.length vs }):
+  Lemma (ensures (R.zip2_lift1 rows 0 vs == R.zip2_cons vs rows))
+        [SMTPat (R.zip2_lift1 rows 0 vs)] =
   match rows, vs with
   | [], [] -> ()
   | _ :: rows', _ :: vs' ->
