src/Pipit.Context.Row.fst
@@ -1,14 +1,15 @@
 (* Rows: contexts are lists of types, and rows are instances of contexts. *)
 module Pipit.Context.Row
 
+module List = FStar.List.Tot
 module C = Pipit.Context.Base
 
-let rec row (l: C.context_t): Type =
+let rec row (l: C.context eqtype): Type =
   match l with
   | [] -> unit
   | t :: ts -> t * row ts
 
-let rec index (l: C.context_t) (r: row l) (i: C.index_lookup l): C.get_index l i =
+let rec index (l: C.context eqtype) (r: row l) (i: C.index_lookup l): C.get_index l i =
   match l with
   | t :: ts ->
     let r': t * row (List.tl l) = r in
@@ -18,39 +19,39 @@ let rec index (l: C.context_t) (r: row l) (i: C.index_lookup l): C.get_index l i
       then r0
       else (
         // Why coerce required?
-        let res: List.index ts (i - 1) = index ts rs (i - 1) in
+        let res: C.get_index ts (i - 1) = index ts rs (i - 1) in
         coerce_eq #_ #(List.index l i) () res)
 
-let rec row_append (r: row 'c) (r': row 'd): row (List.append 'c 'd) =
+let rec append (r: row 'c) (r': row 'd): row (C.append 'c 'd) =
   match 'c with
   | [] -> r'
   | t :: ts ->
     let rr: (t & row ts) = r in
     let (rt, rts) = rr in
-    (rt, row_append rts r')
+    (rt, append rts r')
 
-let row_cons (a: 'a) (r: row 'c): row ('a :: 'c) = (a, r)
+let cons (#a: eqtype) (v: a) (r: row 'c): row (a :: 'c) = (v, r)
 
-let rec row_lift1 (r: row 'c) (i: nat { i <= List.length 'c }) (v: 'a): row (lift1 'c i 'a) =
+let rec lift1 (#a: eqtype) (r: row 'c) (i: C.index_insert 'c) (v: a): row (C.lift1 'c i a) =
   if i = 0 then (v, r)
   else
     match 'c with
     | t :: ts ->
       let rr: (t & row ts) = r in
       let (rt, rts) = rr in
-      (rt, row_lift1 rts (i - 1) v)
+      (rt, lift1 rts (i - 1) v)
 
-let rec row_zip2_append (rs: list (row 'c)) (rs': list (row 'd) { List.length rs == List.length rs' }): list (row (List.append 'c 'd)) =
+let rec zip2_append (rs: list (row 'c)) (rs': list (row 'd) { List.length rs == List.length rs' }): list (row (List.append 'c 'd)) =
   match rs, rs' with
   | [], [] -> []
-  | r :: rs, r' :: rs' -> (row_append r r') :: row_zip2_append rs rs'
+  | r :: rs, r' :: rs' -> (append r r') :: zip2_append rs rs'
 
-let rec row_zip2_cons (rs: list 'a) (rs': list (row 'd) { List.length rs == List.length rs' }): (ret: list (row ('a :: 'd)) { List.length ret == List.length rs }) =
+let rec zip2_cons (#a: eqtype) (rs: list a) (rs': list (row 'd) { List.length rs == List.length rs' }): (ret: list (row (a :: 'd)) { List.length ret == List.length rs }) =
   match rs, rs' with
   | [], [] -> []
-  | r :: rs, r' :: rs' -> (row_cons r r') :: row_zip2_cons rs rs'
+  | r :: rs, r' :: rs' -> (cons r r') :: zip2_cons rs rs'
 
-let rec row_zip2_lift1 (rs: list (row 'c)) (i: nat { i <= List.length 'c }) (vs: list 'a { List.length rs == List.length vs }): (ret: list (row (lift1 'c i 'a)) { List.length ret == List.length rs }) =
+let rec zip2_lift1 (#a: eqtype) (rs: list (row 'c)) (i: C.index_insert 'c) (vs: list a { List.length rs == List.length vs }): (ret: list (row (C.lift1 'c i a)) { List.length ret == List.length rs }) =
   match rs, vs with
   | [], [] -> []
-  | r :: rs, v :: vs -> row_lift1 r i v :: row_zip2_lift1 rs i vs
+  | r :: rs, v :: vs -> lift1 r i v :: zip2_lift1 rs i vs
