src/Pipit.Exp.Base.fst
@@ -1,32 +1,41 @@
 (* Definition of base expression type *)
 module Pipit.Exp.Base
-module C = Pipit.Context
+
 open Pipit.Prim.Table
-open Pipit.Inhabited
 
-(* LATER: restrict "properties" to booleans for now to avoid universe stuff *)
-type xprop = bool
+module C  = Pipit.Context.Base
+module CP = Pipit.Context.Properties
 
+(* Expressions `exp t c a`
+  expressions are indexed by the primitive table, the environment mapping
+  variable indices to value types, and the result type. The primitive table
+  describes the allowed value types and primitive operations. The result type
+  is a `funty` describing a real value type (`FTVal t`) or a partial primitive
+  application (`FTFun arg rest`). Handling primitive applications this way
+  means that we only have one recursive datatype, rather than mutual recursion
+  between this and a list-of-applications, or something. I don't know if it's
+  a good idea or not.
+*)
 noeq
-type exp (t: table) (c: C.context t.typ): funty t.typ -> Type =
+type exp (t: table) (c: context t): funty t.ty -> Type =
   // v
-  | XVal   : a: t.typ -> v: t.typ_sem a -> exp t c (FTVal a)
+  | XVal   : #a: t.ty -> v: t.ty_sem a -> exp t c (FTVal a)
   // bound variable (de Bruijn index)
-  | XBVar  : a: t.typ -> i: C.index { C.opt_index c i == Some (t.typ_sem a) } -> exp t c (FTVal a)
+  | XBVar  : i: C.index_lookup c -> exp t c (FTVal (C.get_index c i))
   // free variables
-  | XVar   : a: t.typ -> x: C.var a -> exp t c (FTVal a)
+  | XVar   : #a: t.ty -> x: C.var a -> exp t c (FTVal a)
   // primitives
-  | XPrim  : p: t.prim -> exp t c (t.prim_types p)
+  | XPrim  : p: t.prim -> exp t c (t.prim_ty p)
   // f(e,...)
-  | XApp   : arg: t.typ -> ret: funty t.typ -> exp t c (FTFun arg ret) -> exp t c [] (FTVal arg) -> exp t c ret
+  | XApp   : #arg: t.ty -> #ret: funty t.ty -> exp t c (FTFun arg ret) -> exp t c (FTVal arg) -> exp t c ret
   // v fby e
-  | XFby   : a: t.typ -> v: a -> exp t c (FTVal a) -> exp t c (FTVal a)
+  | XFby   : #a: t.ty -> v: t.ty_sem a -> exp t c (FTVal a) -> exp t c (FTVal a)
   // e -> e'
-  | XThen  : a: t.typ -> exp c (FTVal a) -> exp c (FTVal a) -> exp c (FTVal a)
+  | XThen  : #a: t.ty -> exp t c (FTVal a) -> exp t c (FTVal a) -> exp t c (FTVal a)
   // µx. e[x]
-  | XMu    : a: t.typ -> exp (a :: c) (FTVal a) -> exp c (FTVal a)
+  | XMu    : #a: t.ty -> exp t (a :: c) (FTVal a) -> exp t c (FTVal a)
   // let x = e in e[x]
-  | XLet   : a: t.typ -> b: t.typ -> exp c (FTVal b) -> exp (b :: c) (FTVal a) -> exp c (FTVal a)
+  | XLet   : #a: t.ty -> b: t.ty -> exp t c (FTVal b) -> exp t (b :: c) (FTVal a) -> exp t c (FTVal a)
 
   // Proof terms
   // Contracts for hiding implementation:
@@ -40,28 +49,31 @@ type exp (t: table) (c: C.context t.typ): funty t.typ -> Type =
   //          exp c 'a
 
   // check "" e
-  | XCheck : string -> exp c xprop -> exp c 'a -> exp c 'a
+  | XCheck : #a: t.ty -> string -> exp t c (FTVal t.propty) -> exp t c (FTVal a) -> exp t c (FTVal a)
 
-let rec weaken (#c c': C.context) (e: exp c 'a): Tot (exp (C.append c c') 'a) (decreases e) =
+let rec weaken (#a: funty ('t).ty) (#c c': context 't) (e: exp 't c a): Tot (exp 't (C.append c c') a) (decreases e) =
   match e with
   | XVal v -> XVal v
   | XBVar i' ->
-    C.lemma_append_preserves_opt_index c c' i';
-    XBVar i'
+    CP.lemma_append_preserves_get_index c c' i';
+    XBVar (i' <: C.index_lookup (C.append c c'))
   | XVar x' -> XVar x'
+  | XPrim p -> XPrim p
   | XApp f e -> XApp (weaken c' f) (weaken c' e)
   | XFby v e -> XFby v (weaken c' e)
   | XThen e1 e2 -> XThen (weaken c' e1) (weaken c' e2)
-  | XMu _ e1 ->
-    let e1': exp (C.append (C.lift1 c 0 'a) c') 'a = weaken c' e1 in
-    let e1'': exp (C.lift1 (C.append c c') 0 'a) 'a = e1' in
-    XMu e1''
+  | XMu e1 ->
+      let e1': exp 't (C.append (C.lift1 c 0 (FTVal?.t a)) c') a = weaken c' e1 in
+      let e1'': exp 't (C.lift1 (C.append c c') 0 (FTVal?.t a)) a = e1' in
+      XMu e1''
   | XLet b e1 e2 -> XLet b (weaken c' e1) (weaken c' e2)
   | XCheck name e1 e2 -> XCheck name (weaken c' e1) (weaken c' e2)
 
 
-let is_base_exp (e: exp 'c 'a): bool = match e with
- | XVal _ | XVar _ | XBVar _ -> true
+let is_base_exp (#c: context 't) (#a: funty ('t).ty) (e: exp 't c a): bool = match e with
+ | XVal _ | XVar _ | XBVar _ | XPrim _ -> true
  | _ -> false
 
-type base_exp (c: C.context) (a: Type) = e : exp c a { is_base_exp e }
+let base_exp (t: table) (c: context t) (a: funty t.ty)  = e: exp t c a { is_base_exp e }
+
+let val_exp (t: table) (c: context t) (a: t.ty) = exp t c (FTVal a)
